Coq/src/SimRelAddCO.v
@@ -12,7 +12,7 @@ From imm Require Import Events Execution
 Require Import AuxRel AuxDef EventStructure BasicStep Step Consistency 
         LblStep CertRf CertGraph EventToAction ImmProperties
         SimRelCont SimRelEventToAction 
-        SimRel SimRelCert SimRelCertBasicStep. 
+        SimRel SimRelCert SimRelCertBasicStep SimRelAddEW. 
 
 Set Implicit Arguments.
 Local Open Scope program_scope.
@@ -68,12 +68,14 @@ Section SimRelAddCO.
 
   Notation "'Stid_' S" := (fun t x => Stid S x = t) (at level 1).
   Notation "'SNTid_' S" := (fun t x => Stid S x <> t) (at level 1).
+  Notation "'SLoc_' S" := (fun l x => Sloc S x = l) (at level 1).
 
   Notation "'GE'" := G.(acts_set).
   Notation "'GEinit'" := (is_init ∩₁ GE).
   Notation "'GEninit'" := ((set_compl is_init) ∩₁ GE).
   Notation "'Glab'" := (G.(lab)).
   Notation "'Gtid'" := (tid).
+  Notation "'Gloc'" := (loc (G.(lab))).
   Notation "'Grmw'" := G.(rmw).
   Notation "'Gaddr'" := G.(addr).
   Notation "'Gdata'" := G.(data).
@@ -118,7 +120,7 @@ Section SimRelAddCO.
     ⟪ wE : SE S w ⟫ /\
     ⟪ wW : SW S w ⟫ /\  
     (* ⟪ wNCF : ~ ES.cont_cf_dom S k w ⟫ /\ *)
-    ⟪ wkSB : dom_rel ((Sco S)^? ⨾ (Sew S)^? ⨾ ⦗set_compl (ES.cont_cf_dom S k)⦘) w ⟫ /\
+    (* ⟪ wkSB : dom_rel ((Sco S)^? ⨾ (Sew S)^? ⨾ ⦗set_compl (ES.cont_cf_dom S k)⦘) w ⟫ /\ *)
     ⟪ wE2Aco : Gco (e2a S w) (e2a S' w') ⟫.
 
   Definition sim_add_co (k : cont_label) (w' : eventid) (S S' : ES.t) : Prop :=
@@ -128,7 +130,8 @@ Section SimRelAddCO.
     (* ⟪ wsW : ws ⊆₁ SW S ⟫ /\ *)
     (* ⟪ wsNCF : ws ∩₁ Scf S' w' ⊆₁ ∅ ⟫ /\ *)
     (* ⟪ wsE : ws ⊆₁ fun w => Gco (e2a S' w) (e2a S' w') ⟫ /\   *)
-    ⟪ CO' : Sco S' ≡ Sco S ∪ ESstep.co_delta (sim_ws k w' S S') w' S ⟫.
+    ⟪ CO' : Sco S' ≡ 
+              Sco S ∪ ESstep.co_delta (sim_ews TC f w' S S') (sim_ws k w' S S') w' S ⟫.
 
   Section SimRelAddCOProps. 
 
@@ -230,35 +233,6 @@ Section SimRelAddCO.
         { apply ES.coD in CO; auto. generalize CO. basic_solver. }
         { apply ES.ewD in EW; auto. generalize EW. basic_solver. }
         apply ES.coD in CO; auto. generalize CO. basic_solver. }
-      { unfolder in CO. unfolder in EW. desf.
-        { destruct wkSB as [a [b [rCO HH]]].
-          assert (Sco S x b) as COxb.
-          { unfolder in rCO. desf.
-            eapply ES.co_trans; eauto. }
-          do 2 eexists; splits; eauto. }
-        { destruct wkSB as [a [b [rCO [c [rEW HH]]]]].
-          unfolder in rCO. unfolder in rEW. desf.
-          { basic_solver 10. }
-          { assert (Sco S z c) as COzc.
-            { eapply ES.ew_co_in_co; eauto. basic_solver. }
-            basic_solver 10. }
-          { assert (Sew S z c) as EWzc.
-            { eapply ES.ew_trans; eauto. }
-            basic_solver 10. }
-          assert (Sco S z c) as COzc.
-          { eapply ES.ew_co_in_co; auto.
-            eexists; splits; eauto.
-            eapply ES.co_ew_in_co; eauto.
-            eexists; splits; eauto. }
-          basic_solver 10. }
-        destruct wkSB as [a [b [rCO HH]]].
-        assert (Sco S x b) as COxb.
-        { unfolder in rCO. desf.
-          { eapply ES.co_ew_in_co; auto. basic_solver 10. }
-          eapply ES.co_trans; eauto.
-          eapply ES.ew_co_in_co; auto.
-          basic_solver. }
-        basic_solver 10. }
       unfolder in CO. unfolder in EW. desf.
       { eapply co_trans; eauto.
         eapply e2a_co; [apply SRCC|].
@@ -275,36 +249,36 @@ Section SimRelAddCO.
       basic_solver 10.
     Qed.
 
-    Lemma sim_ws_basic_step_co_ew_ncf w' k k' e e' S S'
-          (st st' st'' : thread_st (ES.cont_thread S k))
-          (SRCC : simrel_cert prog S G sc TC TC' f h k st st'')
-          (BSTEP_ : ESBasicStep.t_ (thread_lts (ES.cont_thread S k)) k k' st st' e e' S S') 
-          (wEE' : (eq e ∪₁ eq_opt e') w') :
-      sim_ws k w' S S' ⊆₁ dom_rel ((Sco S)^? ⨾ (Sew S)^? ⨾ ⦗set_compl (Scf S' w')⦘).
-    Proof. 
-      cdes BSTEP_.
-      assert (ESBasicStep.t e e' S S') as BSTEP.
-      { econstructor. eauto. }
-      assert (ES.Wf S) as WFS.
-      { apply SRCC. }
-      unfold sim_ws. red. ins. desc.
-      destruct wkSB as [y [a [CO [b [EW [EQ kSB]]]]]].
-      subst b. exists y. 
-      do 2 (eexists; splits; eauto).
-      unfolder; splits; auto.
-      intros CF.
-      eapply ESBasicStep.basic_step_cf in CF; eauto.
-      unfold ESBasicStep.cf_delta in CF.
-      assert (~ SE S w') as nEw'.
-      { red. ins. destruct wEE' as [HA | HB]; desf.
-        { eapply ESBasicStep.basic_step_acts_set_ne; eauto. }
-        unfold eq_opt in HB.
-        destruct e' as [e'|]; desf.
-        eapply ESBasicStep.basic_step_acts_set_ne'; eauto. }
-      unfolder in CF. desf.
-      { apply nEw'. apply ES.cfE, seq_eqv_lr in CF. desf. }
-      all : by (apply nEw'; eapply ES.cont_cf_domE in CF; eauto).
-    Qed.
+    (* Lemma sim_ws_basic_step_co_ew_ncf w' k k' e e' S S' *)
+    (*       (st st' st'' : thread_st (ES.cont_thread S k)) *)
+    (*       (SRCC : simrel_cert prog S G sc TC TC' f h k st st'') *)
+    (*       (BSTEP_ : ESBasicStep.t_ (thread_lts (ES.cont_thread S k)) k k' st st' e e' S S')  *)
+    (*       (wEE' : (eq e ∪₁ eq_opt e') w') : *)
+    (*   sim_ws k w' S S' ⊆₁ dom_rel ((Sco S)^? ⨾ (Sew S)^? ⨾ ⦗set_compl (Scf S' w')⦘). *)
+    (* Proof.  *)
+    (*   cdes BSTEP_. *)
+    (*   assert (ESBasicStep.t e e' S S') as BSTEP. *)
+    (*   { econstructor. eauto. } *)
+    (*   assert (ES.Wf S) as WFS. *)
+    (*   { apply SRCC. } *)
+    (*   unfold sim_ws. red. ins. desc. *)
+    (*   destruct wkSB as [y [a [CO [b [EW [EQ kSB]]]]]]. *)
+    (*   subst b. exists y.  *)
+    (*   do 2 (eexists; splits; eauto). *)
+    (*   unfolder; splits; auto. *)
+    (*   intros CF. *)
+    (*   eapply ESBasicStep.basic_step_cf in CF; eauto. *)
+    (*   unfold ESBasicStep.cf_delta in CF. *)
+    (*   assert (~ SE S w') as nEw'. *)
+    (*   { red. ins. destruct wEE' as [HA | HB]; desf. *)
+    (*     { eapply ESBasicStep.basic_step_acts_set_ne; eauto. } *)
+    (*     unfold eq_opt in HB. *)
+    (*     destruct e' as [e'|]; desf. *)
+    (*     eapply ESBasicStep.basic_step_acts_set_ne'; eauto. } *)
+    (*   unfolder in CF. desf. *)
+    (*   { apply nEw'. apply ES.cfE, seq_eqv_lr in CF. desf. } *)
+    (*   all : by (apply nEw'; eapply ES.cont_cf_domE in CF; eauto). *)
+    (* Qed. *)
 
     (* Lemma sim_ws_basic_step_co_ws w' k k' e e' S S' *)
     (*       (st st' st'' : thread_st (ES.cont_thread S k)) *)
@@ -323,6 +297,98 @@ Section SimRelAddCO.
     (*   all : eauto using  *)
     (*     sim_wsE, sim_wsW, sim_ws_basic_step_nCF, sim_ws_basic_step_loc.  *)
     (* Qed. *)
+
+    Lemma sim_ws_basic_step_ws_Einit w' k k' e e' S S'
+          (st st' st'' : thread_st (ES.cont_thread S k))
+          (SRCC : simrel_cert prog S G sc TC TC' f h k st st'')
+          (BSTEP_ : ESBasicStep.t_ (thread_lts (ES.cont_thread S k)) k k' st st' e e' S S')
+          (SACO : sim_add_co k w' S S')
+          (CST_REACHABLE : (lbl_step (ES.cont_thread S k))＊ st' st'') 
+          (wEE' : (eq e ∪₁ eq_opt e') w') : 
+      SEinit S ∩₁ SLoc_ S (Sloc S' w') ⊆₁ sim_ws k w' S S'.
+    Proof. 
+      cdes BSTEP_; cdes SACO.
+      assert (ESBasicStep.t e e' S S') as BSTEP.
+      { econstructor. eauto. }
+      assert (ES.Wf S) as WFS.
+      { apply SRCC. }
+      assert (Wf G) as WFG.
+      { apply SRCC. }
+      intros x [Init LOCx].
+      assert (SE S x) as SEx.
+      { red in Init. unfolder in Init. desf. }
+      assert (SE S' x) as SEx'.
+      { eapply ESBasicStep.basic_step_acts_set; eauto. basic_solver. }
+      econstructor; splits; auto.
+      { eapply ES.acts_init_set_inW; auto. }
+      eapply init_co_w; auto.
+      { apply SRCC. }
+      { eapply e2a_Einit. 
+        1-2 : apply SRCC. 
+        { eapply e2a_GE. apply SRCC. } 
+        basic_solver. }
+      { intros InitW.
+        assert (~ SEinit S' w') as nInitW.
+        { unfolder in wEE'. desf.
+          { eapply ESBasicStep.basic_step_acts_ninit_set_e; eauto. }
+          eapply ESBasicStep.basic_step_acts_ninit_set_e'; eauto. }
+        apply nInitW.
+        red. split; auto. 
+        etransitivity.
+        { eapply e2a_tid. }
+        unfold tid. unfold is_init in InitW.
+        destruct (e2a S' w'); desf. }
+      { eapply basic_step_e2a_GE; 
+          eauto; try apply SRCC.
+        { admit. }
+        basic_solver. }
+      { unfold is_w. fold (compose Glab (e2a S') w'). 
+        fold (is_w (Glab ∘ e2a S') w').
+        eapply same_lab_u2v_dom_is_w.
+        { apply same_lab_u2v_dom_comm.
+          eapply basic_step_e2a_same_lab_u2v; 
+            eauto; apply SRCC. }
+        basic_solver. }
+      assert 
+        (restr_rel (SE S') (same_loc (Glab ∘ (e2a S'))) x w') 
+        as HH.
+      { eapply same_lab_u2v_dom_same_loc.
+        { apply same_lab_u2v_dom_comm.
+          eapply basic_step_e2a_same_lab_u2v; 
+            eauto; try apply SRCC. }
+        unfolder; splits; eauto.
+        red. arewrite (Sloc S' x = Sloc S x); auto.
+        eapply ESBasicStep.basic_step_loc_eq_dom; eauto. }
+      generalize HH. 
+      unfold same_loc, loc, compose.
+      arewrite (e2a S x = e2a S' x).
+      { symmetry. eapply basic_step_e2a_eq_dom; eauto. }
+      basic_solver.
+    Admitted.
+
+    Lemma sim_ws_basic_step_ews_co_prcl w' k k' e e' S S'
+          (st st' st'' : thread_st (ES.cont_thread S k))
+          (SRCC : simrel_cert prog S G sc TC TC' f h k st st'')
+          (BSTEP_ : ESBasicStep.t_ (thread_lts (ES.cont_thread S k)) k k' st st' e e' S S')
+          (wEE' : (eq e ∪₁ eq_opt e') w') : 
+      dom_rel (Sco S ⨾ ⦗sim_ews TC f w' S S'⦘) ⊆₁ sim_ws k w' S S'.
+    Proof. 
+      cdes BSTEP_.
+      assert (ESBasicStep.t e e' S S') as BSTEP.
+      { econstructor. eauto. }
+      assert (ES.Wf S) as WFS.
+      { apply SRCC. }
+      assert (Wf G) as WFG.
+      { apply SRCC. }
+      intros x [y [z [CO [a SEWS]]]]. 
+      unfold sim_ews in SEWS. desc. subst z.
+      econstructor; splits; auto.
+      { eapply ES.coE in CO; auto. generalize CO. basic_solver. }
+      { eapply ES.coD in CO; auto. generalize CO. basic_solver. }
+      rewrite <- wsE2Aeq.
+      eapply e2a_co; [apply SRCC|].
+      basic_solver 10.
+    Qed.
     
     Lemma weaken_sim_add_co w' k k' e e' S S' 
           (st st' st'' : thread_st (ES.cont_thread S k))
@@ -331,14 +397,15 @@ Section SimRelAddCO.
           (SACO : sim_add_co k w' S S') 
           (CST_REACHABLE : (lbl_step (ES.cont_thread S k))＊ st' st'') 
           (wEE' : (eq e ∪₁ eq_opt e') w') : 
-      ESstep.add_co (sim_ws k w' S S') w' S S'.
+      ESstep.add_co (sim_ews TC f w' S S') (sim_ws k w' S S') w' S S'.
     Proof. 
       cdes BSTEP_; cdes SACO.
       constructor; splits;
         eauto using sim_wsE, sim_wsW, 
           sim_ws_basic_step_loc,
+          sim_ws_basic_step_ws_Einit,
           sim_ws_basic_step_co_ew_prcl,
-          sim_ws_basic_step_co_ew_ncf.
+          sim_ws_basic_step_ews_co_prcl.
     Qed.
     
     (* Lemma basic_step_e2a_co_ws_eq w' k k' e e' S S'  *)
